Basic lemmas, part 1

src/expr.lean
@@ -3,23 +3,100 @@ import defs
 namespace coc
 section
 
+open option
 open idx
 open expr
 
-def expr.update_vars : expr → (nat → idx → expr) → nat → expr
-| (sort s)   f n := sort s
-| (var v)    f n := f n v
-| (app l r)  f n := app (l.update_vars f n) (r.update_vars f n)
-| (lam t e)  f n := lam (t.update_vars f n) (e.update_vars f (n + 1))
-| (pi t₁ t₂) f n := pi (t₁.update_vars f n) (t₂.update_vars f (n + 1))
+def imax : nat → nat → nat
+| 0 _ := 0
+| _ 0 := 0
+| a b := max a b
+
+def expr.size : expr → nat
+| (sort s)   := 1
+| (var v)    := 1
+| (app l r)  := (l.size + r.size).succ
+| (lam t e)  := (t.size + e.size).succ
+| (pi t₁ t₂) := (t₁.size + t₂.size).succ
+
+def expr.closed : expr → nat → Prop
+| (sort s)        n := true
+| (var (bound b)) n := b < n
+| (var (free f))  n := true
+| (app l r)       n := expr.closed l n ∧ expr.closed r n
+| (lam t e)       n := expr.closed t n ∧ expr.closed e n.succ
+| (pi t₁ t₂)      n := expr.closed t₁ n ∧ expr.closed t₂ n.succ
+
+structure cexpr (n : nat) : Type :=
+  (e : expr) (hce : expr.closed e n)
 
 /-- Make a free variable into an "overflowed" bound variable. -/
-def expr.make_bound : expr → nat → expr
-| e s := e.update_vars (λ n x, if x = free s then var (bound n) else var x) 0
+@[irreducible]
+def expr.bind : expr → nat → nat → expr
+| (sort s)   n f := sort s
+| (var v)    n f := if v = free f then var (bound n) else var v
+| (app l r)  n f := app (expr.bind l n f) (expr.bind r n f)
+| (lam t e)  n f := lam (expr.bind t n f) (expr.bind e n.succ f)
+| (pi t₁ t₂) n f := pi (expr.bind t₁ n f) (expr.bind t₂ n.succ f)
 
 /-- Replace one overflow variable by an expression. -/
-def expr.make_replace : expr → expr → expr
-| e t := e.update_vars (λ n x, if x = bound n then t else var x) 0
+@[irreducible]
+def expr.subs : expr → nat → expr → expr
+| (sort s)   n e' := sort s
+| (var v)    n e' := if v = bound n then e' else var v
+| (app l r)  n e' := app (expr.subs l n e') (expr.subs r n e')
+| (lam t e)  n e' := lam (expr.subs t n e') (expr.subs e n.succ e')
+| (pi t₁ t₂) n e' := pi (expr.subs t₁ n e') (expr.subs t₂ n.succ e')
+
+/-- Small-step reduction rules. -/
+inductive small : expr → expr → Prop
+| s_beta      {t e r}     : small (app (lam t e) r) (e.subs 0 r)
+| s_app_left  {l l' r}    : small l l' →   small (app l r) (app l' r)
+| s_app_right {l r r'}    : small r r' →   small (app l r) (app l r')
+| s_lam_left  {t t' e}    : small t t' →   small (lam t e) (lam t' e)
+| s_lam_right {t e e'}    : small e e' →   small (lam t e) (lam t e')
+| s_pi_left   {t₁ t₁' t₂} : small t₁ t₁' → small (pi t₁ t₂) (pi t₁' t₂)
+| s_pi_right  {t₁ t₂ t₂'} : small t₂ t₂' → small (pi t₁ t₂) (pi t₁ t₂')
+
+/-- Transitive closure of small-step reduction rules. -/
+inductive small_star : expr → expr → Prop
+| ss_refl {e}        :                                    small_star e e
+| ss_step {e₁ e₂ e₃} : small_star e₁ e₂ → (small e₂ e₃) → small_star e₁ e₃
+
+/-- Symmetric transitive closure of small-step reduction rules. -/
+inductive small_eq : expr → expr → Prop
+| ss_refl {e}        :                                  small_eq e e
+| ss_symm {e₁ e₂}    : small_eq e₁ e₂ →                 small_eq e₂ e₁
+| ss_step {e₁ e₂ e₃} : small_eq e₁ e₂ → (small e₂ e₃) → small_eq e₁ e₃
+
+/-- Typing rules (without free variables). -/
+inductive has_type : ctx → expr → expr → Prop
+| t_conv {Γ e t t'} :
+  small_eq t t' →
+  has_type Γ e t →
+  has_type Γ e t'
+| t_sort {Γ n} :
+  has_type Γ (sort n) (sort n.succ)
+| t_var {Γ n t} :
+  list.nth Γ n = some t →
+  has_type Γ (var (bound n)) t
+| t_app {Γ l r t₁ t₂} :
+  has_type Γ l (pi t₁ t₂) →
+  has_type Γ r t₁ →
+  has_type Γ (app l r) (t₂.subs 0 r)
+| t_lam {Γ t₁ t₂ s e} :
+  has_type Γ (pi t₁ t₂) (sort s) →
+  has_type (t₁ :: Γ) e t₂ →
+  has_type Γ (lam t₁ e) (pi t₁ t₂)
+| t_pi {Γ t₁ s₁ t₂ s₂} :
+  has_type Γ t₁ (sort s₁) →
+  has_type (t₁ :: Γ) t₂ (sort s₂) →
+  has_type Γ (pi t₁ t₂) (sort (imax s₁ s₂))
+
+/-- Rules for defining well-formed local contexts. -/
+inductive ctx_wf : ctx → Prop
+| c_nil          :                                    ctx_wf []
+| c_cons {Γ t s} : ctx_wf Γ → has_type Γ t (sort s) → ctx_wf (t :: Γ)
 
 /-- Performs applicative-order beta-reduction.
     If the original expression is well-typed, the resulting expression will have the same type.
@@ -32,18 +109,11 @@ meta def expr.reduce : expr → expr
   let l := l.reduce,
       r := r.reduce
   in match l with
-  | (lam _ lr) := (lr.make_replace r).reduce 
-  | _          := app l r
+  | (lam t e) := (e.subs 0 r).reduce
+  | _         := app l r
   end
 | (lam t e)  := lam t.reduce e.reduce
 | (pi t₁ t₂) := pi t₁.reduce t₂.reduce
-
-def expr.size : expr → int
-| (sort s)   := 1
-| (var v)    := 1
-| (app l r)  := l.size + r.size + 1
-| (lam t e)  := t.size + e.size + 1
-| (pi t₁ t₂) := t₁.size + t₂.size + 1
 
 end
 end coc
