src/checker.lean
@@ -7,11 +7,6 @@ open idx
 open expr
 open ctx
 
-def expr.imax : nat → nat → nat
-| 0 _ := 0
-| _ 0 := 0
-| a b := max a b
-
 def expr.as_sort : expr → string ⊕ nat
 | (sort s) := sum.inr s
 | e        := sum.inl $ "expression " ++ e.show ++ " is not a sort"
@@ -20,14 +15,10 @@ def expr.as_pi : expr → string ⊕ (expr × expr)
 | (pi t₁ t₂) := sum.inr (t₁, t₂)
 | e          := sum.inl $ "expression " ++ e.show ++ " is not a function"
 
-def ctx.length : ctx → nat
-| nil        := nat.zero
-| (cons _ Γ) := nat.succ (ctx.length Γ)
-
-def ctx.nth : ctx → nat → string ⊕ expr
-| nil        _       := sum.inl "undefined variable"
-| (cons t Γ) 0       := sum.inr t
-| (cons t Γ) (n + 1) := ctx.nth Γ n
+def ctx.try_nth : ctx → nat → string ⊕ expr
+| []       _       := sum.inl "undefined variable"
+| (t :: Γ) 0       := sum.inr t
+| (t :: Γ) (n + 1) := ctx.try_nth Γ n
 
 /-- Check if a preterm is a well-formed term (1), type (2), proof (3) or formula (4).
     (1) Returns a well-formed expression of type `sort (n + 1)`, representing the type of the term;
@@ -36,28 +27,28 @@ def ctx.nth : ctx → nat → string ⊕ expr
     (4) Returns `sort 0` itself. -/
 meta def expr.check_rec : expr → Π (Γ Δ : ctx), string ⊕ expr
 | (sort s)        Γ Δ := return (sort (s + 1))
-| (var (bound b)) Γ Δ := Δ.nth b
-| (var (free f))  Γ Δ := Γ.nth (Γ.length - 1 - f)
+| (var (bound b)) Γ Δ := Δ.try_nth b
+| (var (free f))  Γ Δ := Γ.try_nth (Γ.length - 1 - f)
 | (app l r)   Γ Δ := do
   { tl        ← l.check_rec Γ Δ,
     ⟨t₁, t₂⟩  ← tl.as_pi,
     tr        ← r.check_rec Γ Δ,
     if t₁.reduce = tr.reduce
-    then return (t₂.make_replace r)
+    then return (t₂.subs 0 r)
     else sum.inl $ "argument type mismatch: " ++ t₁.show ++ " != " ++ tr.show }
 | (lam t e)   Γ Δ := do
   { t'        ← t.check_rec Γ Δ,
     _         ← t'.as_sort,
-    t₂        ← e.check_rec Γ (cons t Δ),
+    t₂        ← e.check_rec Γ (t :: Δ),
     return (pi t t₂) }
 | (pi t₁ t₂)  Γ Δ := do
   { t'        ← t₁.check_rec Γ Δ,
     s₁        ← t'.as_sort,
-    t''       ← t₂.check_rec Γ (cons t₁ Δ),
+    t''       ← t₂.check_rec Γ (t₁ :: Δ),
     s₂        ← t''.as_sort,
-    return (sort (expr.imax s₁ s₂)) }
+    return (sort (imax s₁ s₂)) }
 
 meta def expr.check (e : expr) (Γ : ctx) : string ⊕ expr :=
-  e.check_rec Γ nil
+  e.check_rec Γ []
 
 end coc
