src/lemmas.lean
@@ -1,0 +1,125 @@
+import tactic
+import expr
+
+namespace coc
+section
+
+set_option pp.structure_projections false
+
+open option
+open idx
+open expr
+
+local notation e `⟦` r `/$⟧`    := subs e 0 r
+local notation e ` ~> ` e'      := small e e'
+local notation e ` ~>* ` e'     := small_star e e'
+local notation Γ ` ⊢ ` e `: ` t := has_type Γ e t
+local notation `⊢ ` Γ           := ctx_wf Γ
+
+namespace closed
+
+  /-- Lemmas for `closed e n`: `e` has at most `n` levels of unbound variables. -/
+  lemma c_sort (s n)                                                  : closed (sort s) n        := trivial
+  lemma c_bound {b n} (h : b < n)                                     : closed (var (bound b)) n := h
+  lemma c_free (f n)                                                  : closed (var (free f)) n  := trivial
+  lemma c_app {l r n} (hcl : closed l n) (hcr : closed r n)           : closed (app l r) n       := ⟨hcl, hcr⟩
+  lemma c_lam {t e n} (hct : closed t n) (hce : closed e n.succ)      : closed (lam t e) n       := ⟨hct, hce⟩
+  lemma c_pi {t₁ t₂ n} (hct₁ : closed t₁ n) (hct₂ : closed t₂ n.succ) : closed (pi t₁ t₂) n      := ⟨hct₁, hct₂⟩
+
+  lemma c_weaken {e n n'} (hce : closed e n) (h : n <= n') : closed e n' :=
+    @expr.rec (λ e, ∀ n n', n ≤ n' → closed e n → closed e n')
+      (λ _ _ _ _ _, c_sort _ _)
+      (λ v _ _ h,
+        match v with
+        | (bound b) := λ hcb, c_bound (nat.lt_of_lt_of_le hcb h)
+        | (free f) := λ hcf, c_free _ _
+        end)
+      (λ _ _ hl hr _ _ h ⟨hcl, hcr⟩, ⟨hl _ _ h hcl, hr _ _ h hcr⟩)
+      (λ _ _ ht he _ _ h ⟨hct, hce⟩, ⟨ht _ _ h hct, he _ _ (nat.succ_le_succ h) hce⟩)
+      (λ _ _ ht₁ ht₂ _ _ h ⟨hct₁, hct₂⟩, ⟨ht₁ _ _ h hct₁, ht₂ _ _ (nat.succ_le_succ h) hct₂⟩)
+      e n n' h hce
+
+  lemma c_weaken₁ {e n} (hce : closed e n) : closed e n.succ :=
+    c_weaken hce (nat.le_succ n)
+
+end closed
+open closed
+
+/-- Substitution at the topmost level "closes" that level of unbound variables. -/
+lemma subs.close {e e'} {n : nat} :
+  closed e n.succ → closed e' n → closed (subs e n e') n := by
+{ intros hce hce',
+  induction e generalizing n,
+  case sort : s { unfold subs },
+  case var : v
+  { unfold subs,
+    cases v with b f,
+    { change b < n.succ at hce,
+      split_ifs with hif; injections; contradiction <|> skip,
+      exact nat.lt_of_le_and_ne (nat.le_of_lt_succ hce) h, },
+    { split_ifs; injections } },
+  case app : l r hl hr { unfold subs, exact c_app (hl hce.1 hce') (hr hce.2 hce') },
+  case lam : t e ht he { unfold subs, exact c_lam (ht hce.1 hce') (he hce.2 (c_weaken₁ hce')) },
+  case pi : t₁ t₂ ht₁ ht₂ { unfold subs, exact c_lam (ht₁ hce.1 hce') (ht₂ hce.2 (c_weaken₁ hce')) } }
+
+/-- Substitution at the topmost level 0 makes the term closed. -/
+lemma subs.close₀ {e e'} : closed e 1 → closed e' 0 → closed (subs e 0 e') 0 :=
+  subs.close
+
+/-- `red1 e₁ e₂`: `e₁` reduces to `e₂` by contracting zero or more immediate, disjoint redexes. -/
+inductive red1 : expr → expr → Prop
+| r1_beta {t e r}         : red1 (app (lam t e) r) (e.subs 0 r)
+| r1_sort (s)             :                             red1 (sort s) (sort s)
+| r1_var  (v)             :                             red1 (var v) (var v)
+| r1_app  {l l' r r'}     : red1 l l' → red1 r r' →     red1 (app l r) (app l' r')
+| r1_lam  {t t' e e'}     : red1 t t' → red1 e e' →     red1 (lam t e) (lam t' e')
+| r1_pi   {t₁ t₁' t₂ t₂'} : red1 t₁ t₁' → red1 t₂ t₂' → red1 (pi t₁ t₂) (pi t₁' t₂')
+open red1
+
+local notation e ` ~>₁ ` e' := red1 e e'
+
+lemma red1.refl (e : expr) : e ~>₁ e :=
+  @expr.rec_on (λ e, e ~>₁ e) e
+    r1_sort r1_var (λ _ _, r1_app) (λ _ _, r1_lam) (λ _ _, r1_pi)
+
+lemma red1.of_red1_left_rep
+  {e e' e₁ : expr}
+  (hce : closed e 0) (hce' : closed e' 0) (hce₁ : closed e₁ 0)
+  (h : e ~>₁ e') :
+  e⟦e₁/$⟧ ~>₁ e'⟦e₁/$⟧ := by
+{ induction h,
+  case r1_beta : t e r
+  {  },
+  case r1_sort : h
+  { admit },
+  case r1_var : h
+  { admit },
+  case r1_app : h_l h_l' h_r h_r' h_ᾰ h_ᾰ_1 h_ih_ᾰ h_ih_ᾰ_1
+  { admit },
+  case r1_lam : h_t h_t' h_e h_e' h_ᾰ h_ᾰ_1 h_ih_ᾰ h_ih_ᾰ_1
+  { admit },
+  case r1_pi : h_t₁ h_t₁' h_t₂ h_t₂' h_ᾰ h_ᾰ_1 h_ih_ᾰ h_ih_ᾰ_1
+  { admit }}
+
+lemma red1.confluent {e e₁ e₂ : expr} (h₁ : e ~>₁ e₁) (h₂ : e ~>₁ e₂) :
+  ∃ e', (e₁ ~>₁ e') ∧ (e₂ ~>₁ e') := by
+{ induction e generalizing e₁ e₂,
+  case sort : s { cases h₁, cases h₂, use (sort s), exact ⟨r1_sort s, r1_sort s⟩, },
+  case var : v { cases h₁, cases h₂, use (var v), exact ⟨r1_var v, r1_var v⟩ },
+  case app : l r ihl ihr
+  { cases h₁,
+    case r1_app : l l₁ r r₁ hl₁ hr₁
+    { cases h₂,
+      case r1_beta : t e r
+      { rcases hl₁ with _ | _ | _ | _ | @⟨t, t', e, e', ht, he⟩ | _,
+        use e'.subs 0 r,
+         },
+      case r1_app : l l₂ r r₂ hl₂ hr₂
+      { cases ihl hl₁ hl₂ with el hel,
+        cases ihr hr₁ hr₂ with er her,
+        use (app el er), exact ⟨r1_app hel.1 her.1, r1_app hel.2 her.2⟩ }}
+  }
+}
+
+end
+end coc
