src/main.lean
@@ -15,22 +15,21 @@ def prop := sort 0
 def type := sort 1
 def bin := λ a f b, app (app f a) b
 
-def c₁ :=
-  ⟦(pi (fv 0) $ pi (fv 0) prop)⟧ :: -- [13] mem       : setvar → setvar → Prop
-  ⟦(pi (pi (fv 0) prop) prop)  ⟧ :: -- [12] unique    : (setvar → Prop) → Prop
-  ⟦(pi (pi (fv 0) prop) prop)  ⟧ :: -- [11] exists    : (setvar → Prop) → Prop
-  ⟦(pi (pi (fv 0) prop) prop)  ⟧ :: -- [10] forall    : (setvar → Prop) → Prop
-  ⟦(pi prop $ pi prop prop)    ⟧ :: -- [9]  iff       : Prop → Prop → Prop
-  ⟦(pi prop $ pi prop prop)    ⟧ :: -- [8]  implies   : Prop → Prop → Prop
-  ⟦(pi prop $ pi prop prop)    ⟧ :: -- [7]  or        : Prop → Prop → Prop
-  ⟦(pi prop $ pi prop prop)    ⟧ :: -- [6]  and       : Prop → Prop → Prop
-  ⟦(pi prop prop)              ⟧ :: -- [5]  not       : Prop → Prop
-  ⟦prop                        ⟧ :: -- [4]  false     : Prop
-  ⟦prop                        ⟧ :: -- [3]  true      : Prop
-  ⟦(pi (fv 0) $ pi (fv 0) prop)⟧ :: -- [2]  equals    : setvar → setvar → Prop
-  ⟦(fv 0)                      ⟧ :: -- [1]  arbitrary : setvar 
-  ⟦type                        ⟧ :: -- [0]  setvar    : Type
-  nil
+def c₁ : ctx :=
+  [ (pi (fv 0) $ pi (fv 0) prop), -- [13] mem       : setvar → setvar → Prop
+    (pi (pi (fv 0) prop) prop),   -- [12] unique    : (setvar → Prop) → Prop
+    (pi (pi (fv 0) prop) prop),   -- [11] exists    : (setvar → Prop) → Prop
+    (pi (pi (fv 0) prop) prop),   -- [10] forall    : (setvar → Prop) → Prop
+    (pi prop $ pi prop prop),     -- [9]  iff       : Prop → Prop → Prop
+    (pi prop $ pi prop prop),     -- [8]  implies   : Prop → Prop → Prop
+    (pi prop $ pi prop prop),     -- [7]  or        : Prop → Prop → Prop
+    (pi prop $ pi prop prop),     -- [6]  and       : Prop → Prop → Prop
+    (pi prop prop),               -- [5]  not       : Prop → Prop
+    prop,                         -- [4]  false     : Prop
+    prop,                         -- [3]  true      : Prop
+    (pi (fv 0) $ pi (fv 0) prop), -- [2]  equals    : setvar → setvar → Prop
+    (fv 0),                       -- [1]  arbitrary : setvar
+    type ]                        -- [0]  setvar    : Type
 
 def and := fv 6
 def iff := fv 9
@@ -46,7 +45,7 @@ def e₁ :=
             and (app (app (bv 3) (bv 2)) (bv 0))))))
 
 meta def main : io unit := do
-{ io.put_str_ln c₁.show,
+{ io.put_str_ln c₁.to_string,
   io.put_str_ln e₁.show,
   io.put_str_ln "",
   match e₁.check c₁ with
